SN Proof of ECC
git-svn-id: svn+ssh://scm.gforge.inria.fr/svn/coqcert/trunk/cic-model@185 7b0040dd-6dd6-45fd-888d-7922243e4794

GenModelSN.v
@@ -185,6 +185,13 @@ unfold eq_typ; split; simpl; intros.
  rewrite H; rewrite H0; eauto.
 Qed.
 
+Lemma assume_wf e M T :
+  (wf e -> typ e M T) ->
+  typ e M T.
+red; intros; apply H; trivial.
+red; eauto.
+Qed.
+
 (** * Strong normalization *)
 
 (* This lemma shows that the abstract model construction entails
@@ -233,6 +240,34 @@ destruct H.
  red; intros; trivial.
 Qed.
 
+Definition type_ok e T :=
+  T <> kind /\ forall i j, val_ok e i j -> Lc.sn (tm j T) /\ exists w, w ∈ int i T.
+
+Lemma typs_type_ok e T :
+  wf e -> typs e T -> type_ok e T.
+intros (i0,(j0,is_val0)) ty_T.
+split; intros.
+ destruct ty_T as [ty_T|ty_T]; apply ty_T in is_val0; destruct is_val0; trivial.
+
+ split.
+  destruct ty_T as [ty_T|ty_T]; apply ty_T in H; apply in_int_sn in H; trivial.
+
+  apply typs_kind_ok with (1:=ty_T) (2:=H).
+Qed.
+
+Lemma typs_is_non_empty e i j T :
+  typs e T ->
+  val_ok e i j -> 
+  T <> kind /\ Lc.sn (tm j T) /\ exists w, w ∈ int i T.
+split.
+ apply typs_not_kind with (2:=H).
+ exists i; exists j; trivial.
+split.
+ destruct H; apply H in H0; apply in_int_sn in H0; trivial.
+
+ apply typs_kind_ok with (1:=H) (2:=H0).
+Qed.
+
 (** #<a name="MakeModel.TypingRules"></a># *)
 
 (** * Inference rules *)
@@ -244,6 +279,16 @@ red.
 exists vnil; exists (fun _ => SatSet.daimon).
 red; intros.
 destruct n; discriminate.
+Qed.
+
+Lemma wf_cons_ok : forall e T,
+  wf e ->
+  type_ok e T ->
+  wf (T::e).
+unfold wf; intros e T (i,(j,is_val)) (T_nk,inh_T).
+destruct inh_T with (1:=is_val) as (_,(x,non_mt)).
+exists (V.cons x i); exists (I.cons SatSet.daimon j).
+apply vcons_add_var0; trivial.
 Qed.
 
 Lemma wf_cons : forall e T,
@@ -387,16 +432,13 @@ apply prod_elim with (x:=int i v) in H1; trivial.
  rewrite H4; reflexivity.
 Qed.
 
-Lemma typ_abs : forall e T M U,
-  typs e T ->
+Lemma typ_abs_ok : forall e T M U,
+  type_ok e T ->
   typ (T :: e) M U ->
   U <> kind ->
   typ e (Abs T M) (Prod T U).
 Proof.
-intros e T M U ty_T ty_M not_tops i j is_val.
-assert (T_not_tops : T <> kind).
- destruct ty_T as [ty_T|ty_T]; apply ty_T in is_val;
-   destruct is_val; trivial.
+intros e T M U (T_not_tops,inh_T) ty_M not_tops i j is_val.
 apply in_int_intro; simpl; try discriminate.
  apply prod_intro; intros.
   red; intros.
@@ -411,23 +453,45 @@ apply in_int_intro; simpl; try discriminate.
   destruct is_val; trivial.
 
  rewrite Real_prod.
- destruct (typs_kind_ok ty_T is_val) as (wit,in_T).
- apply KSAT_intro.
-  destruct ty_T as [ty_T|ty_T]; apply ty_T in is_val;
-    destruct is_val as (_,(_,satT)); simpl in satT; trivial.
-  rewrite Real_sort in satT; trivial.
+ specialize inh_T with (1:=is_val).
+ destruct inh_T as (snT, (wit, in_T)).
+ apply KSAT_intro; trivial.
+ apply prodSAT_intro; intros.
+ apply interSAT_intro; intros.
+  exists wit; trivial.
 
-  apply prodSAT_intro; intros.
-  apply interSAT_intro; intros.
-   exists wit; trivial.
+  destruct x; simpl in *.
+  assert (val_ok (T::e) (V.cons x i) (I.cons v j)).
+   apply vcons_add_var; auto.
+  apply ty_M in H0.
+  apply in_int_not_kind in H0; trivial.
+  destruct H0 as (_,H0).
+  rewrite <- tm_subst_cons; trivial.
+Qed.
 
-   destruct x; simpl in *.
-   assert (val_ok (T::e) (V.cons x i) (I.cons v j)).
-    apply vcons_add_var; auto.
-   apply ty_M in H0.
-   apply in_int_not_kind in H0; trivial.
-   destruct H0 as (_,H0).
-   rewrite <- tm_subst_cons; trivial.
+Lemma typ_abs : forall e T M U,
+  typs e T ->
+  typ (T :: e) M U ->
+  U <> kind ->
+  typ e (Abs T M) (Prod T U).
+Proof.
+intros e T M U ty_T ty_M not_tops.
+apply assume_wf; intro wfe.
+apply typ_abs_ok; trivial.
+apply typs_type_ok; trivial.
+Qed.
+
+Lemma typ_beta_ok : forall e T M N U,
+  type_ok e T ->
+  typ (T::e) M U ->
+  typ e N T ->
+  T <> kind ->
+  U <> kind ->
+  typ e (App (Abs T M) N) (subst N U).
+Proof.
+intros.
+apply typ_app with T; trivial.
+apply typ_abs_ok; trivial.
 Qed.
 
 Lemma typ_beta : forall e T M N U,
@@ -443,45 +507,25 @@ apply typ_app with T; trivial.
 apply typ_abs; trivial.
 Qed.
 
-Lemma typ_prod : forall e T U s2,
-  s2 = kind \/ s2 = prop ->
-  typs e T ->
-  typ (T :: e) U s2 ->
-  typ e (Prod T U) s2.
+Lemma typ_prod_prop : forall e T U,
+  type_ok e T ->
+  typ (T :: e) U prop ->
+  typ e (Prod T U) prop.
 Proof.
-intros e T U s2 is_srt ty_T ty_U i j is_val.
-assert (T_not_tops : T <> kind).
- destruct ty_T as [ty_T|ty_T]; apply ty_T in is_val;
-   destruct is_val; trivial.
-assert (typs (T::e) U) by (destruct is_srt; subst; red; auto).
-destruct (typs_kind_ok ty_T is_val) as (witT,in_T).
+intros e T U (T_not_tops, inh_T) ty_U i j is_val.
+specialize inh_T with (1:=is_val).
+destruct inh_T as (snT,(witT, in_T)).
 specialize vcons_add_var0 with (1:=is_val) (2:=in_T) (3:=T_not_tops);
   intros in_U.
 apply ty_U in in_U.
-assert (Lc.sn (tm j T)).
- destruct ty_T as [ty_T|ty_T]; apply ty_T in is_val;
-   destruct is_val as (_,(_,satT)); trivial.
- apply sat_sn in satT; trivial.
-split;[discriminate|destruct is_srt; subst s2; split;simpl].
- (* s2=kind *)
- (* kind_ok: *)
- apply prod_kind_ok.
- destruct in_U as (_,(mem,_)); trivial.
-
- (* sn *)
- destruct in_U as (_,(_,satU)).
- rewrite tm_subst_cons in satU.
- apply Lc.sn_subst in satU.
- apply KSAT_intro with (A:=snSAT); auto.
-
- (* s2=prop *)
+split;[discriminate|split;simpl].
  (* value *)
  apply impredicative_prod; intros.   
   red; intros.
-  rewrite H2; reflexivity.
+  rewrite H0; reflexivity.
 
   clear in_U.
-  specialize vcons_add_var0 with (1:=is_val) (2:=H1) (3:=T_not_tops);
+  specialize vcons_add_var0 with (1:=is_val) (2:=H) (3:=T_not_tops);
     intros in_U.
   apply ty_U in in_U.
   apply in_int_not_kind in in_U;[|discriminate].
@@ -493,6 +537,47 @@ split;[discriminate|destruct is_srt; subst s2; split;simpl].
  rewrite tm_subst_cons in satU.
  apply Lc.sn_subst in satU.
  apply KSAT_intro with (A:=snSAT); auto.
+Qed.
+
+Lemma typ_prod : forall e T U s2,
+  s2 = kind \/ s2 = prop ->
+  typs e T ->
+  typ (T :: e) U s2 ->
+  typ e (Prod T U) s2.
+Proof.
+intros e T U s2 is_srt ty_T ty_U.
+destruct is_srt; subst s2.
+ (* s2=kind *)
+ intros i j is_val.
+ assert (T_not_tops : T <> kind).
+  destruct ty_T as [ty_T|ty_T]; apply ty_T in is_val;
+    destruct is_val; trivial.
+ destruct (typs_kind_ok ty_T is_val) as (witT,in_T).
+ specialize vcons_add_var0 with (1:=is_val) (2:=in_T) (3:=T_not_tops);
+   intros in_U.
+ apply ty_U in in_U.
+ assert (Lc.sn (tm j T)).
+  destruct ty_T as [ty_T|ty_T]; apply ty_T in is_val;
+    destruct is_val as (_,(_,satT)); trivial.
+  apply sat_sn in satT; trivial.
+ split;[discriminate|split;simpl].
+  (* kind_ok: *)
+  apply prod_kind_ok.
+  destruct in_U as (_,(mem,_)); trivial.
+
+  (* sn *)
+  destruct in_U as (_,(_,satU)).
+  rewrite tm_subst_cons in satU.
+  apply Lc.sn_subst in satU.
+  apply KSAT_intro with (A:=snSAT); auto.
+
+ (* s2=prop *)
+ apply assume_wf; intros (i0,(j0,is_val0)).
+ destruct typs_is_non_empty with (1:=ty_T) (2:=is_val0) as (T_nk,_).
+ apply typ_prod_prop; trivial.
+ split; trivial.
+ intros.
+ destruct typs_is_non_empty with (1:=ty_T) (2:=H); trivial.
 Qed.
 
 Lemma typ_conv : forall e M T T',
