SN_ECC.v
@@ -1,0 +1,1262 @@
+Require Export Relations Wellfounded Compare_dec.
+Require Import Sat.
+Require Import ZF ZFcoc ZFecc.
+Require Import ZFlambda.
+
+(** Strong normalization proof of the Extended Calculus of Constructions.
+    It is based on GenModelSN, so it does not support strong eliminations.
+    Inhabitation of all types is obtained by adding the empty set in every
+    type. The product is interpreted by the set of *partial* functions.
+ *)
+
+Set Implicit Arguments.
+
+(***********************************************************************)
+(** * Proving the SN requirements *)
+
+Module CCSN.
+
+Definition mkTY x S := couple x (iSAT S).
+Definition Elt T := fst T. (* total elements *)
+Definition El T := union2 (singl empty) (Elt T). (* partial elements *)
+Definition Real T := sSAT (snd T) .
+
+Lemma Elt_El x y : x ∈ Elt y -> x ∈ El y.
+intros; apply union2_intro2; trivial.
+Qed.
+Lemma empty_El y : empty ∈ El y.
+apply union2_intro1; apply singl_intro.
+Qed.
+Hint Resolve Elt_El empty_El.
+
+Definition piSAT A (F:set->SAT) :=
+  prodSAT (Real A) (interSAT (fun p:{y|y ∈ El A} => F (proj1_sig p))).
+
+Definition sn_prod A F :=
+  mkTY (cc_prod (El A) (fun x => El (F x)))
+       (piSAT A (fun x => Real (F x))).
+
+Definition sn_lam A F := cc_lam (El A) F.
+
+Lemma sn_prod_intro0 : forall dom f F,
+  ext_fun (El dom) f ->
+  ext_fun (El dom) F ->
+  (forall x, x ∈ El dom -> f x ∈ El (F x)) ->
+  sn_lam dom f ∈ Elt (sn_prod dom F).
+unfold sn_lam, sn_prod, mkTY, El, Elt.
+intros.
+rewrite fst_def.
+apply cc_prod_intro; intros; auto.
+do 2 red; intros.
+apply union2_morph; auto with *.
+apply fst_morph; auto.
+Qed.
+Lemma sn_prod_intro : forall dom f F,
+  ext_fun (El dom) f ->
+  ext_fun (El dom) F ->
+  (forall x, x ∈ El dom -> f x ∈ El (F x)) ->
+  sn_lam dom f ∈ El (sn_prod dom F).
+intros.
+apply Elt_El.
+apply sn_prod_intro0; auto.
+Qed.
+
+Lemma sn_prod_elim : forall dom f x F,
+  f ∈ El (sn_prod dom F) ->
+  x ∈ El dom ->
+  cc_app f x ∈ El (F x).
+intros.
+unfold sn_prod, mkTY, El in H.
+apply union2_elim in H; destruct H.
+ apply singl_elim in H.
+ rewrite H.
+ rewrite cc_app_empty; auto.
+
+ unfold Elt at 1 in H; rewrite fst_def in H.
+ apply cc_prod_elim with (dom:=El dom) (F:=fun x => El(F x)); trivial.
+(*
+ apply union2_elim in H0; destruct H0.
+  apply singl_elim in H0.
+  assert (x ∈ Elt dom \/ ~ x ∈ Elt dom). admit.
+  destruct H1.
+   apply cc_prod_elim with (dom:=Elt dom) (F:=fun x => El(F x)); trivial.
+
+   assert (cc_app f x == empty).
+    apply empty_ext.
+    red; intros y ?.
+    rewrite <- couple_in_app in H2.
+    apply H1.
+    apply cc_prod_is_cc_fun in H.
+    red in H.
+    apply H in H2.
+    destruct H2 as (_,?).
+    rewrite fst_def in H2; trivial.
+   rewrite H2; auto.
+
+  apply cc_prod_elim with (dom:=Elt dom) (F:=fun x => El(F x)); trivial.*)
+Qed.
+
+Lemma cc_impredicative_prod_non_empty : forall dom F,
+  ext_fun dom F ->
+  (forall x, x ∈ dom -> F x == singl prf_trm) ->
+  cc_prod dom F == singl prf_trm.
+Proof.
+intros.
+apply singl_ext; intros.
+ rewrite <- (cc_impredicative_lam dom (fun x => prf_trm)); intros.
+ 2:do 2 red; reflexivity.
+  apply cc_prod_intro; intros; auto.
+  apply H0 in H1; rewrite H1.
+  apply singl_intro.
+
+  reflexivity.
+
+ unfold cc_prod in H1.
+ rewrite replf_ax in H1; intros.
+  destruct H1 as (f,f_fun,z_lam).
+  rewrite z_lam; clear z z_lam.
+  apply cc_impredicative_lam; intros.
+   do 2 red; intros.
+   rewrite H2; reflexivity.
+
+   apply singl_elim.
+   fold prf_trm.
+   rewrite <- (H0 _ H1).
+   apply dep_func_elim with (1:=f_fun); trivial.
+
+  do 2 red; intros.
+  apply cc_lam_ext; try reflexivity.
+  red; intros.
+  apply app_morph; trivial.
+Qed.
+
+
+Definition sn_props :=
+  mkTY (replSAT(fun A => mkTY (singl prf_trm) A)) snSAT.
+
+Lemma prop_repl_morph :
+  Proper (eqSAT ==> eq_set) (fun A => mkTY (singl prf_trm) A).
+do 2 red; intros.
+apply couple_morph; try reflexivity.
+apply iSAT_morph; trivial.
+Qed.
+Hint Resolve prop_repl_morph.
+
+Lemma sn_impredicative_prod : forall dom F,
+  ext_fun (El dom) F ->
+  (forall x, x ∈ El dom -> F x ∈ El sn_props) ->
+  sn_prod dom F ∈ El sn_props.
+intros.
+apply Elt_El.
+unfold sn_props, mkTY, El, Elt in *.
+rewrite fst_def.
+assert (singl prf_trm ∈ props).
+ apply power_intro; auto.
+rewrite replSAT_ax; trivial.
+exists (piSAT dom (fun x : set => Real (F x))).
+unfold sn_prod, mkTY.
+apply couple_morph; auto with *.
+apply cc_impredicative_prod_non_empty.
+ do 2 red; intros; unfold El, Elt.
+ apply union2_morph; auto with *.
+ apply fst_morph.
+ apply H; trivial.
+(* apply union2_intro2; trivial.*)
+
+ intros.
+ specialize H0 with (1:=H2).
+ rewrite fst_def in H0.
+ apply union2_elim in H0; destruct H0.
+  apply singl_elim in H0.
+  unfold El; rewrite H0.
+  apply eq_intro; intros.
+   apply union2_elim in H3; destruct H3; trivial.
+   unfold Elt, fst in H3.
+   apply union_elim in H3; destruct H3.
+   apply subset_elim1 in H4.
+   rewrite union_empty_eq in H4.
+   apply empty_ax in H4; contradiction.
+
+   apply union2_intro1; trivial.
+
+  rewrite replSAT_ax in H0; trivial.
+  destruct H0.
+  unfold El; rewrite H0; rewrite fst_def.
+  apply eq_intro; intros.
+   apply union2_elim in H3; destruct H3; trivial.
+   apply union2_intro1; trivial.
+Qed.
+
+(*
+
+Definition sn_props :=
+  mkTY (sup props (fun P => replSAT(fun A => mkTY P A))) snSAT.
+
+Lemma prop_repl_morph :
+  Proper (eq_set ==> eqSAT ==> eq_set) (fun P A => mkTY P A).
+do 3 red; intros.
+apply couple_morph; trivial.
+apply iSAT_morph; trivial.
+Qed.
+Lemma prop_repl_morph2 :
+  Proper (eq_set ==> eq_set) (fun P => replSAT(fun A => mkTY P A)).
+do 2 red; intros.
+apply ZFrepl.repl_morph_raw; auto with *.
+do 2 red; intros.
+rewrite H1.
+unfold mkTY; rewrite H.
+rewrite (iSAT_morph _ _ (sSAT_morph _ _ H0)).
+reflexivity.
+Qed.
+Hint Resolve prop_repl_morph prop_repl_morph2.
+
+Lemma sn_impredicative_prod : forall dom F,
+  ext_fun (El dom) F ->
+  (forall x, x ∈ El dom -> F x ∈ El sn_props) ->
+  sn_prod dom F ∈ El sn_props.
+intros.
+apply Elt_El.
+unfold sn_props, mkTY, El, Elt in *.
+rewrite fst_def.
+pose (P := cc_prod (Elt dom) (fun x => El(F x))).
+assert (P ∈ props).
+ apply cc_impredicative_prod; intros.
+ specialize H0 with (1:=Elt_El H1).
+ rewrite fst_def in H0.
+ apply power_intro; intros.
+ apply union2_elim in H2; destruct H2; trivial.
+ apply union2_elim in H0; destruct H0.
+  apply singl_elim in H0.
+  rewrite H0 in H2.
+  unfold Elt, fst in H2.
+  apply union_elim in H2; destruct H2.
+  apply subset_elim1 in H3.
+  rewrite union_empty_eq in H3.
+  apply empty_ax in H3; contradiction.
+
+  rewrite sup_ax in H0.
+  2:do 2 red; intros; apply prop_repl_morph2; auto.
+  destruct H0.
+  rewrite replSAT_ax in H3.
+  2:apply prop_repl_morph; reflexivity.
+  destruct H3.
+  rewrite H3 in H2.
+  unfold Elt in H2; rewrite fst_def in H2.
+  apply power_elim with x0; auto.
+rewrite sup_ax.
+2:do 2 red; intros; apply prop_repl_morph2; auto.
+exists P; auto with *.
+rewrite replSAT_ax; trivial.
+2:apply prop_repl_morph; reflexivity.
+exists (piSAT dom (fun x : set => Real (F x))).
+reflexivity.
+Qed.
+*)
+
+  Lemma sn_proof_of_false : prf_trm ∈ El (sn_prod sn_props (fun P => P)).
+auto.
+(*
+setoid_replace prf_trm with (cc_lam (El sn_props) (fun _ => prf_trm)).
+ unfold sn_prod, mkTY, El; rewrite fst_def.
+ apply cc_prod_intro; intros.
+  do 2 red; reflexivity.
+
+  do 2 red; intros; apply fst_morph; trivial.
+  unfold sn_props, mkTY in H.
+  rewrite fst_def in H.
+  rewrite replSAT_ax in H; trivial.
+  destruct H as (A, eq_x).
+  rewrite eq_x.
+  rewrite fst_def.
+  apply singl_intro.
+
+ symmetry.
+ apply cc_impredicative_lam; intros.
+  do 2 red; intros; reflexivity.
+  reflexivity.*)
+Qed.
+
+End CCSN.
+Import CCSN.
+
+(** * Building the CC abstract SN model *)
+
+
+Require Import Models.
+Module SN_CC_Model <: CC_Model.
+
+Definition X := set.
+Definition inX x y := x ∈ El y.
+Definition eqX := eq_set.
+Lemma eqX_equiv : Equivalence eqX.
+Proof eq_set_equiv.
+
+Lemma in_ext: Proper (eqX ==> eqX ==> iff) inX.
+do 3 red; intros.
+unfold inX, El, eqX in *.
+rewrite H; rewrite H0; reflexivity.
+Qed.
+
+Definition props := sn_props.
+Definition app := cc_app.
+Definition lam := sn_lam.
+Definition prod := sn_prod.
+(*
+Notation "x ∈ y" := (inX x y).
+Notation "x == y" := (eqX x y).
+*)
+Definition eq_fun (x:X) (f1 f2:X->X) :=
+  forall y1 y2, inX y1 x -> y1 == y2 -> f1 y1 == f2 y2.
+
+Lemma eq_fun_El x f1 f2 : eq_fun x f1 f2 -> ZF.eq_fun (El x) f1 f2.
+do 2 red; intros.
+apply H; auto.
+Qed.
+Hint Resolve eq_fun_El.
+
+Lemma lam_ext :
+  forall x1 x2 f1 f2,
+  x1 == x2 ->
+  eq_fun x1 f1 f2 ->
+  lam x1 f1 == lam x2 f2.
+unfold lam, sn_lam, eqX; intros.
+apply cc_lam_ext; auto.
+unfold El; rewrite H; reflexivity.
+Qed.
+
+Lemma app_ext: Proper (eqX ==> eqX ==> eqX) app.
+Proof cc_app_morph.
+
+Lemma prod_ext :
+  forall x1 x2 f1 f2,
+  x1 == x2 ->
+  eq_fun x1 f1 f2 ->
+  prod x1 f1 == prod x2 f2.
+unfold prod, sn_prod, eqX, mkTY, El; intros.
+apply couple_morph.
+ apply cc_prod_ext; intros.
+  rewrite H; reflexivity.
+
+  red; intros.
+  apply union2_morph; auto with *.
+  apply fst_morph; apply H0; auto.
+  red; auto.
+
+ apply iSAT_morph.
+ unfold piSAT, Real.
+ apply prodSAT_morph.
+  apply sSAT_morph; apply snd_morph; trivial.
+
+  apply interSAT_morph_subset; simpl; intros.
+   unfold El; rewrite H; reflexivity.
+
+   apply sSAT_morph; apply snd_morph; apply H0; auto; reflexivity.
+Qed.
+
+Lemma prod_intro : forall dom f F,
+  eq_fun dom f f ->
+  eq_fun dom F F ->
+  (forall x, inX x dom -> inX (f x) (F x)) ->
+  inX (lam dom f) (prod dom F).
+Proof sn_prod_intro.
+
+Lemma prod_elim : forall dom f x F,
+  eq_fun dom F F ->
+  inX f (prod dom F) ->
+  inX x dom ->
+  inX (app f x) (F x).
+intros.
+eapply sn_prod_elim; eauto.
+Qed.
+
+Lemma impredicative_prod : forall dom F,
+  eq_fun dom F F ->
+  (forall x, inX x dom -> inX (F x) props) ->
+  inX (prod dom F) props.
+Proof sn_impredicative_prod.
+
+Lemma beta_eq:
+  forall dom F x,
+  eq_fun dom F F ->
+  inX x dom ->
+  app (lam dom F) x == F x.
+unfold app, lam, inX, eqX; intros.
+apply cc_beta_eq; auto.
+Qed.
+
+End SN_CC_Model.
+
+Import SN_CC_Model.
+
+(***********************************************************************)
+(** Building the SN addon *)
+
+Module SN_CC_addon.
+
+  Definition Real : X -> SAT := Real.
+
+  Lemma Real_morph : Proper (eqX ==> eqSAT) Real.
+do 2 red; intros.
+apply sSAT_morph.
+apply snd_morph; trivial.
+Qed.
+
+  Lemma Real_sort : eqSAT (Real props) snSAT.
+unfold Real, CCSN.Real, props, sn_props, mkTY.
+rewrite snd_def.
+rewrite iSAT_id.
+reflexivity.
+Qed.
+
+  Lemma Real_prod : forall A B,
+    eqSAT (Real (prod A B))
+     (prodSAT (Real A)
+        (interSAT (fun p:{y|inX y A} => Real (B (proj1_sig p))))).
+unfold Real, CCSN.Real, prod, sn_prod, piSAT, mkTY; intros.
+rewrite snd_def.
+rewrite iSAT_id.
+reflexivity.
+Qed.
+
+  Definition daimon := empty.
+
+  Lemma daimon_false : inX daimon (prod props (fun P => P)).
+Proof sn_proof_of_false.
+
+End SN_CC_addon.
+
+
+(** * Universes *)
+
+Definition sort K :=
+  sup K (fun P => replSAT (fun A => mkTY P A)).
+
+Lemma sort_repl_morph :
+  Proper (eq_set ==> eqSAT ==> eq_set) (fun P A => mkTY P A).
+do 3 red; intros.
+apply couple_morph; trivial.
+apply iSAT_morph; trivial.
+Qed.
+Lemma sort_repl_morph2 :
+  Proper (eq_set ==> eq_set) (fun P => replSAT(fun A => mkTY P A)).
+do 2 red; intros.
+apply ZFrepl.repl_morph_raw; auto with *.
+do 2 red; intros.
+rewrite H1.
+unfold mkTY; rewrite H.
+rewrite (iSAT_morph _ _ (sSAT_morph _ _ H0)).
+reflexivity.
+Qed.
+Hint Resolve sort_repl_morph sort_repl_morph2.
+
+
+Definition sn_type n := mkTY (sort (ecc n)) snSAT.
+
+Import ZFgrothendieck.
+Hint Resolve ecc_grot.
+
+
+Lemma omega_ecc0 : ZFord.omega ⊆ ecc 0.
+red; intros.
+unfold ZFord.omega, ZFord.ord_sup in H.
+rewrite sup_ax in H.
+ destruct H.
+ rewrite ZFrepl.uchoice_ax in H0.
+  destruct H0.
+  destruct H0.
+  rewrite <- H2 in H1.
+  apply G_trans with (ZFord.nat2ordset x1); trivial.
+  elim x1; intros.
+   apply G_incl with ZFcoc.props; trivial.
+    apply ecc_in1.
+    red; intros.
+    apply empty_ax in H3; contradiction.
+
+   apply G_subset; trivial.
+   apply G_power; auto.
+
+  (* Fch *)
+  split;[|split]; intros.
+ revert H2; apply ex2_morph; red; intros; auto with *.
+ rewrite H1; reflexivity.
+
+ elim H using ZFnats.N_ind; intros.
+  revert H3; apply ex_morph.
+  red; intros.
+  apply ex2_morph; red; intros; auto with *.
+  rewrite H2; reflexivity.
+
+  exists (ZFord.nat2ordset 0); exists 0; simpl; auto with *.
+
+  destruct H2 as (y,(m,?,?)).
+  exists (ZFord.nat2ordset (S m)); exists (S m); simpl; auto with *.
+  apply ZFnats.succ_morph; trivial.
+
+ destruct H1; destruct H2.
+ rewrite <- H3; rewrite <- H4; rewrite H1 in H2; apply ZFnats.nat2set_inj in H2.
+ rewrite H2; reflexivity.
+
+ (* Fm *)
+do 2 red; intros.
+apply ZFrepl.uchoice_morph_raw.
+red; intros.
+apply ex2_morph.
+ red; intros.
+ rewrite H1; reflexivity.
+
+ red; intros.
+ rewrite H2; reflexivity.
+Qed.
+
+Lemma omega_in_ecc1 : ZFord.omega ∈ ecc 1.
+apply G_incl with (ecc 0); auto.
+ apply grot_succ_in; exact gr.
+
+ apply omega_ecc0.
+Qed.
+
+(* ecc 0 is countable so we need to skip it.
+   ecc 1 is not countable...*)
+Lemma CCLam_ecc0 : CCLam ∈ ecc 1.
+unfold CCLam.
+unfold Lam.Lambda.
+apply G_TI; auto.
+ do 2 red; intros.
+ unfold Lam.LAMf.
+ rewrite H; reflexivity.
+
+ apply omega_in_ecc1.
+
+ intros.
+ unfold Lam.LAMf.
+ apply G_union2; trivial.
+  apply G_union2; trivial.
+   apply G_prodcart; trivial.
+    apply G_singl; trivial.
+    apply G_trans with ZFnats.N; auto.
+    apply ZFnats.zero_typ.
+    apply G_N; trivial.
+    apply omega_in_ecc1.
+
+    apply G_N; trivial.
+    apply omega_in_ecc1.
+
+   apply G_prodcart; trivial.
+    apply G_singl; trivial.
+    apply G_trans with ZFnats.N; auto.
+    apply ZFnats.succ_typ.
+    apply ZFnats.zero_typ.
+    apply G_N; trivial.
+    apply omega_in_ecc1.
+
+    apply G_trans with ZFnats.N; auto.
+    apply ZFnats.zero_typ.
+    apply G_N; trivial.
+    apply omega_in_ecc1.
+
+  apply G_union2; trivial.
+   apply G_prodcart; trivial.
+    apply G_singl; trivial.
+    apply G_trans with ZFnats.N; auto.
+    apply ZFnats.succ_typ.
+    apply ZFnats.succ_typ.
+    apply ZFnats.zero_typ.
+    apply G_N; trivial.
+    apply omega_in_ecc1.
+
+    apply G_prodcart; trivial.
+
+   apply G_prodcart; trivial.
+    apply G_singl; trivial.
+    apply G_trans with ZFnats.N; auto.
+    apply ZFnats.succ_typ.
+    apply ZFnats.succ_typ.
+    apply ZFnats.succ_typ.
+    apply ZFnats.zero_typ.
+    apply G_N; trivial.
+    apply omega_in_ecc1.
+Qed.
+Hint Resolve CCLam_ecc0.
+
+Lemma ecc_incl_le x m n :
+  le m n -> x ∈ ecc m -> x ∈ ecc n.
+induction 1; intros; auto with *.
+apply ecc_incl; auto.
+Qed.
+(*
+Lemma G_props n : ZFcoc.props.gl empty ∈ ecc n.
+apply G_singl; trivial.
+apply G_incl with ZFcoc.props; trivial.
+ apply ecc_in1.
+cl_le with (m:=0); auto with *.
+ apply ecc_in.
+*)
+
+Lemma G_TY T A n :
+  T ∈ ecc (S n) ->
+  mkTY T A ∈ ecc (S n).
+intros.
+unfold mkTY.
+apply G_couple; trivial.
+apply G_subset; auto.
+apply ecc_incl_le with 1; auto with *.
+Qed.
+
+Lemma sort_intro K T A :
+  T ∈ K -> mkTY T A ∈ sort K.
+intros.
+unfold sort.
+rewrite sup_ax; auto.
+exists T; trivial.
+rewrite replSAT_ax; auto.
+2:apply sort_repl_morph; reflexivity.
+exists A; reflexivity.
+Qed.
+
+Lemma sort_elim_raw K T : T ∈ sort K -> exists U A, T == mkTY U A /\ U ∈ K.
+unfold sort; rewrite sup_ax; auto.
+intros (U,?,?).
+rewrite replSAT_ax in H0.
+2:apply sort_repl_morph; reflexivity.
+destruct H0 as (A,?).
+eauto.
+Qed.
+
+Lemma sort_elim K T : T ∈ sort K -> Elt T ∈ K.
+intros.
+apply sort_elim_raw in H; destruct H as (U,(A,(?,?))).
+rewrite H.
+unfold Elt, mkTY; rewrite fst_def; trivial.
+Qed.
+
+Lemma sn_prop_type0 :
+  inX sn_props (sn_type 1).
+apply Elt_El.
+unfold Elt, sn_type, mkTY; rewrite fst_def.
+apply sort_intro.
+apply G_replf; auto.
+ do 2 red; intros; apply couple_morph; auto with *.
+ apply iSAT_morph; apply sSAT_morph; trivial.
+
+ apply G_power; trivial.
+
+ intros.
+ unfold mkTY.
+ apply G_couple; trivial.
+  apply G_trans with ZFcoc.props; auto.
+   apply power_intro; auto.
+   apply ecc_in1.
+
+  apply G_subset; auto.
+Qed.
+
+Lemma sn_type_type n :
+  inX (sn_type n) (sn_type (S n)).
+apply Elt_El.
+unfold Elt, sn_type, mkTY; rewrite fst_def.
+apply sort_intro.
+apply G_sup; auto.
+ apply ecc_in2.
+
+ intros.
+ apply G_replf; auto.
+  do 2 red; intros; apply couple_morph; auto with *.
+  apply iSAT_morph; apply sSAT_morph; trivial.
+
+  apply G_power; trivial.
+  apply ecc_incl_le with 1; auto with *.
+
+  intros.
+  unfold mkTY.
+  apply G_couple; trivial.
+   apply ecc_incl; trivial.
+
+   apply G_subset; auto.
+   apply ecc_incl_le with 1; auto with *.
+Qed.
+
+Lemma El_type n T :
+  T ∈ singl empty ∪ sort (ecc n) ->
+  El T ∈ ecc n.
+intros.
+apply union2_elim in H; destruct H.
+ apply G_union2; trivial.
+  apply G_trans with ZFcoc.props; auto.
+   apply power_intro; auto.
+   apply ecc_in1.
+
+   apply singl_elim in H.
+   rewrite H.
+   apply G_union; trivial.
+   apply G_subset; trivial.
+   apply G_union; trivial.
+   apply G_incl with ZFcoc.props; auto.
+    apply ecc_in1.
+    red; intros.
+    apply empty_ax in H0; contradiction.
+
+  apply sort_elim in H.
+  apply G_union2; auto.
+  apply G_trans with ZFcoc.props; auto.
+   apply power_intro; auto.
+   apply ecc_in1.
+Qed.
+
+Lemma sn_predicative_prod : forall n dom F,
+  ext_fun (El dom) F ->
+  dom ∈ El (sn_type n) ->
+  (forall x, x ∈ El dom -> F x ∈ El (sn_type n)) ->
+  sn_prod dom F ∈ El (sn_type n).
+intros.
+apply Elt_El.
+unfold sn_type, mkTY, El, Elt in *.
+rewrite fst_def in H0|-*.
+apply sort_intro.
+apply ecc_prod; intros.
+ do 2 red; intros.
+ apply union2_morph; auto with *.
+ apply fst_morph.
+ apply H; auto.
+
+ apply El_type; trivial.
+
+ specialize H1 with (1:=H2).
+ rewrite fst_def in H1.
+ apply El_type; trivial.
+Qed.
+
+
+(***********************************************************************)
+(*
+----
+*)
+
+Require GenModelSN.
+Module SN := GenModelSN.MakeModel SN_CC_Model SN_CC_addon.
+
+(** ** Extendability *)
+Definition cst (x:set) : SN.trm.
+left; exists (fun _ =>x) (fun _ =>Lambda.K).
+ do 2 red; reflexivity.
+ do 2 red; reflexivity.
+ red; reflexivity.
+ red; reflexivity.
+Defined.
+
+Definition mkSET (x:set) := cst (mkTY x snSAT).
+
+Lemma mkSET_kind e x :
+(*  (exists w, in_set w x) ->*)
+  SN.typ e (mkSET x) SN.kind.
+red; intros.
+split;[discriminate|].
+split;[|apply Lambda.sn_K].
+exists nil; exists (mkSET x).
+ reflexivity.
+
+ exists empty; simpl; intros _.
+ apply union2_intro1.
+ apply singl_intro.
+Qed.
+
+Lemma cst_typ e x y :
+  in_set x y ->
+  SN.typ e (cst x) (mkSET y).
+red; intros.
+apply SN.in_int_intro; try discriminate.
+ simpl.
+ apply Elt_El.
+ unfold mkTY, Elt.
+ rewrite fst_def; trivial. 
+
+ unfold SN_CC_addon.Real, Real, SN.tm, SN.int, mkSET, cst, SN.iint, SN.itm.
+ unfold mkTY; rewrite snd_def.
+ rewrite iSAT_id.
+ apply Lambda.sn_K.
+Qed.
+(*
+Lemma cst_typ_inv x y :
+  SN.typ nil (cst x) (mkSET y) ->
+  in_set x y.
+intros.
+assert (SN.val_ok nil (SN.V.nil empty) (SN.I.nil Lambda.K)).
+ red; intros.
+ destruct n; inversion H0.
+apply H in H0.
+apply SN.in_int_not_kind in H0.
+2:discriminate.
+destruct H0 as (H0,_ ); simpl in H0.
+unfold SN_CC_Model.inX, mkTY, El in H0.
+rewrite fst_def in H0; trivial.
+Qed.
+*)
+Lemma cst_eq_typ e x y :
+  x == y ->
+  SN.eq_typ e (cst x) (cst y).
+red; simpl; intros; trivial.
+Qed.
+
+Lemma cst_eq_typ_inv x y :
+  SN.eq_typ nil (cst x) (cst y) ->
+  x == y.
+intros.
+assert (SN.val_ok nil (SN.V.nil empty) (SN.I.nil Lambda.K)).
+ red; intros.
+ destruct n; inversion H0.
+apply H in H0.
+simpl in H0; trivial.
+Qed.
+
+Lemma mkSET_eq_typ e x y :
+  x == y ->
+  SN.eq_typ e (mkSET x) (mkSET y).
+red; simpl; intros; trivial.
+unfold mkTY; rewrite H; reflexivity.
+Qed.
+
+Lemma mkSET_eq_typ_inv x y :
+  SN.eq_typ nil (mkSET x) (mkSET y) ->
+  x == y.
+intros.
+assert (SN.val_ok nil (SN.V.nil empty) (SN.I.nil Lambda.K)).
+ red; intros.
+ destruct n; inversion H0.
+apply H in H0.
+simpl in H0; trivial.
+apply couple_injection in H0; destruct H0; trivial.
+Qed.
+
+(** * Predicative universes: inference rules *)
+
+Definition type (n:nat) : SN.trm := cst (sn_type (S n)).
+
+Lemma typ_prop_type0 e :
+  SN.typ e SN.prop (type 0).
+red; intros.
+apply SN.in_int_intro.
+ apply sn_prop_type0.
+
+ simpl SN.int; simpl SN.tm.
+ simpl SN_CC_addon.Real.
+ unfold SN_CC_addon.Real, sn_type.
+ unfold Real, mkTY.
+ generalize (snSAT_intro Lambda.sn_K).
+ apply inSAT_morph; auto.
+ rewrite snd_def.
+ rewrite iSAT_id; reflexivity.
+
+ discriminate.
+ discriminate.
+Qed.
+
+Lemma typ_type_type e n :
+  SN.typ e (type n) (type (S n)).
+red; intros.
+apply SN.in_int_intro.
+ apply sn_type_type.
+
+ simpl SN.int; simpl SN.tm.
+ simpl SN_CC_addon.Real.
+ unfold SN_CC_addon.Real, sn_type.
+ unfold Real, mkTY.
+ generalize (snSAT_intro Lambda.sn_K).
+ apply inSAT_morph; auto.
+ rewrite snd_def.
+ rewrite iSAT_id; reflexivity.
+
+ discriminate.
+ discriminate.
+Qed.
+
+Lemma typ_prop_cumul e T :
+  SN.typ e T SN.prop ->
+  SN.typ e T (type 0).
+red; intros.
+apply H in H0.
+destruct H0.
+split; trivial.
+destruct H1.
+split.
+ revert H1; apply union2_mono; auto with *.
+Opaque ecc.
+ simpl; unfold props, sn_props, sn_type; simpl.
+ unfold Elt, mkTY; rewrite fst_def; rewrite fst_def.
+ red; intros.
+ rewrite replSAT_ax in H1.
+ 2:apply prop_repl_morph.
+ destruct H1.
+ rewrite H1.
+ apply sort_intro.
+ apply ecc_incl.
+ apply ecc_incl_prop.
+ apply power_intro; auto.
+
+ revert H2; apply inSAT_morph; trivial.
+ apply sSAT_morph.
+ simpl; unfold props, sn_props, sn_type, mkTY.
+ rewrite snd_def; rewrite snd_def; reflexivity.
+Qed.
+
+Lemma typ_type_cumul e T n :
+  SN.typ e T (type n) ->
+  SN.typ e T (type (S n)).
+red; intros.
+apply H in H0.
+destruct H0.
+split; trivial.
+destruct H1.
+split.
+ revert H1; apply union2_mono; auto with *.
+ unfold Elt, type, sn_type, mkTY; simpl.
+ rewrite fst_def; rewrite fst_def.
+ red; intros.
+ apply sort_elim_raw in H1.
+ destruct H1 as (U,(A,(?,?))).
+ rewrite H1; apply sort_intro.
+ revert H3; apply (ecc_incl (S n)).
+
+ revert H2; apply inSAT_morph; trivial.
+ apply sSAT_morph.
+ simpl; unfold sn_type, mkTY.
+ rewrite snd_def; rewrite snd_def; reflexivity.
+Qed.
+Lemma typ_type_cumul_le e T m n :
+  le m n ->
+  SN.typ e T (type m) ->
+  SN.typ e T (type n).
+induction 1; intros; auto.
+apply typ_type_cumul; auto.
+Qed.
+
+Lemma typ_predicative_prod e T U n :
+  SN.typ e T (type n) ->
+  SN.typ (T::e) U (type n) ->
+  SN.typ e (SN.Prod T U) (type n).
+unfold SN.typ; intros.
+specialize H with (1:=H1).
+destruct H as (?,(?,?)); trivial.
+split;[discriminate|].
+split.
+ apply sn_predicative_prod; trivial.
+  red; red; intros.
+  rewrite H5; reflexivity.
+
+  intros.
+  specialize SN.vcons_add_var0 with (1:=H1) (2:=H4) (3:=H);
+    intros in_U.
+  apply H0 in in_U.
+  apply SN.in_int_not_kind in in_U;[|discriminate].
+  destruct in_U; trivial.
+
+  assert (forall i, eqSAT (SN_CC_addon.Real (SN.int i (type n))) snSAT).
+   simpl; intros _.
+   unfold SN_CC_addon.Real, sn_type, Real, mkTY.
+   rewrite snd_def.
+   rewrite iSAT_id; reflexivity.
+  specialize SN.vcons_add_var0 with (1:=H1) (2:=empty_El _) (3:=H);
+    intros in_U.
+  apply H0 in in_U.
+  destruct in_U  as (_,(_,satU)).
+  rewrite H4 in H3,satU|-*.
+  simpl in satU|-*.
+  rewrite SN.tm_subst_cons in satU.
+  apply Lambda.sn_subst in satU.
+  apply KSAT_intro with (A:=snSAT); auto.
+Qed.
+
+(** * Mapping from syntactic entities to their semantic counterparts. *)
+
+(** syntax of ECC *)
+Require TypeJudgeECC.
+Module Ty := TypeJudgeECC.
+Module Tm := TermECC.
+Module Lc := Lambda.
+
+
+(** Terms *)
+Fixpoint int_trm t :=
+  match t with
+  | Tm.Srt Tm.prop => SN.prop
+  | Tm.Srt (Tm.kind n) => type n
+  | Tm.Ref n => SN.Ref n
+  | Tm.App u v => SN.App (int_trm u) (int_trm v)
+  | Tm.Abs T M => SN.Abs (int_trm T) (int_trm M)
+  | Tm.Prod T U => SN.Prod (int_trm T) (int_trm U)
+  end.
+Definition interp t := int_trm t.
+Definition int_env := List.map interp.
+
+Section LiftAndSubstEquiv.
+(* Proof that lift and subst at both levels (SN and Tm) are equivalent. *)
+
+(* Locally Import this module *)
+Import SN.
+
+Lemma int_lift_rec : forall n t k,
+  eq_trm (lift_rec n k (int_trm t)) (int_trm (Tm.lift_rec n t k)).
+induction t; simpl int_trm; intros.
+ destruct s; simpl; trivial.
+ split; red; intros; reflexivity.
+
+ split; red; intros; reflexivity.
+
+ simpl; unfold V.lams, I.lams, V.shift, I.shift.
+ destruct (le_gt_dec k n0); simpl.
+  replace (k+(n+(n0-k))) with (n+n0) by omega.
+  split; red; auto.
+
+  split; red; auto.
+
+ rewrite red_lift_abs; rewrite IHt1; rewrite IHt2; reflexivity.
+ rewrite red_lift_app; rewrite IHt1; rewrite IHt2; reflexivity.
+ rewrite red_lift_prod; rewrite IHt1; rewrite IHt2; reflexivity.
+Qed.
+
+Lemma int_lift : forall n t,
+  eq_trm (int_trm (Tm.lift n t)) (lift n (int_trm t)).
+intros.
+symmetry.
+unfold Tm.lift, lift.
+apply int_lift_rec.
+Qed.
+
+Lemma int_subst_rec : forall arg,
+  int_trm arg <> kind ->
+  forall t k,
+  eq_trm (subst_rec (int_trm arg) k (int_trm t)) (int_trm (Tm.subst_rec arg t k)).
+intros arg not_knd.
+induction t; simpl int_trm; intros.
+ destruct s; simpl; trivial.
+ split; red; intros; reflexivity.
+
+ split; red; intros; reflexivity.
+
+ simpl Tm.subst_rec.
+ destruct (lt_eq_lt_dec k n) as [[fv|eqv]|bv]; simpl int_trm.
+  simpl int_trm.
+  destruct n; [inversion fv|].
+  rewrite SN.red_sigma_var_gt; auto with arith.
+  reflexivity.
+
+  subst k; rewrite SN.red_sigma_var_eq; trivial.
+  symmetry; apply int_lift.
+
+  rewrite SN.red_sigma_var_lt; trivial.
+  reflexivity.
+
+ rewrite SN.red_sigma_abs.
+ rewrite IHt1; rewrite IHt2; reflexivity.
+
+ rewrite SN.red_sigma_app.
+ rewrite IHt1; rewrite IHt2; reflexivity.
+
+ rewrite SN.red_sigma_prod.
+ rewrite IHt1; rewrite IHt2; reflexivity.
+Qed.
+
+
+Lemma int_subst : forall u t,
+  int_trm u <> kind ->
+  eq_trm (int_trm (Tm.subst u t)) (subst (int_trm u) (int_trm t)).
+unfold Tm.subst; symmetry; apply int_subst_rec; trivial.
+Qed.
+
+End LiftAndSubstEquiv.
+(* Proof that beta-reduction at the Lc level simulates beta-reduction
+   at the Tm level. One beta at the Tm level may require several
+   (but not zero) steps at the Lc level, because of the encoding
+   of type-carrying lambda abstractions.
+ *)
+Lemma red1_sound : forall x y,
+  Tm.red1 x y ->
+  SN.red_term (int_trm x) (int_trm y).
+induction 1; simpl; intros.
+ rewrite int_subst.
+  apply SN.red_term_beta.
+
+  destruct N; try discriminate.
+  destruct s; try discriminate.
+
+ apply SN.red_term_abs_l; auto 10.
+ apply SN.red_term_abs_r; auto 10.
+ apply SN.red_term_app_l; auto 10.
+ apply SN.red_term_app_r; auto 10.
+ apply SN.red_term_prod_l; auto 10.
+ apply SN.red_term_prod_r; auto 10.
+Qed.
+
+Lemma sn_sound : forall M,
+  Acc (transp _ SN.red_term) (interp M) ->
+  Tm.sn M.
+intros M accM.
+apply Acc_inverse_image with (f:=int_trm) in accM.
+induction accM; intros.
+constructor; intros.
+apply H0; trivial.
+ apply red1_sound; trivial.
+Qed.
+
+
+(** Soundness of the typing rules *)
+
+Lemma interp_nk : forall T, interp T <> SN.kind.
+induction T; simpl; intros; try discriminate.
+destruct s; discriminate.
+Qed.
+Hint Resolve interp_nk.
+
+Lemma typ_sort_type_ok e T s : 
+  T <> SN.kind ->
+  SN.typ e T (interp (TermECC.Srt s)) ->
+  SN.type_ok e T.
+split; trivial.
+split.
+ apply H0 in H1.
+ apply SN.in_int_sn in H1; trivial.
+
+ exists empty; red; auto. 
+Qed.
+
+Lemma int_sound : forall e M M' T,
+  Ty.eq_typ e M M' T ->
+  SN.typ (int_env e) (interp M) (interp T) /\
+  SN.eq_typ (int_env e) (interp M) (interp M').
+induction 1; simpl; intros.
+ (* Srt *)
+ split.
+  apply typ_prop_type0.
+  apply SN.refl.
+ split.
+  apply typ_type_type.
+  apply SN.refl.
+ (* Ref *)
+ split.
+  destruct H0.
+  subst t.
+  unfold Tm.lift, interp.
+  fold (Tm.lift (S v) x); rewrite int_lift.
+  simpl.
+  apply SN.typ_var.
+  elim H1; simpl; auto.
+
+  apply SN.refl.
+ (* Abs *)
+ destruct IHeq_typ1.
+ clear IHeq_typ2.
+ destruct IHeq_typ3.
+ unfold interp; simpl; fold (interp T) (interp M) (interp U).
+ split.
+  apply SN.typ_abs_ok; eauto.
+  apply typ_sort_type_ok in H3; auto.
+
+  apply SN.eq_typ_abs; eauto.
+ (* App *)
+ destruct IHeq_typ1.
+ destruct IHeq_typ3.
+ clear IHeq_typ2 IHeq_typ4.
+ unfold interp; simpl; fold (interp u) (interp v) (interp Ur).
+ split.
+  rewrite int_subst; fold (interp v); eauto.
+  fold (interp Ur).
+  apply SN.typ_app with (interp V); eauto.
+
+  apply SN.eq_typ_app; trivial.
+ (* Prod *)
+ destruct IHeq_typ1.
+ destruct IHeq_typ2.
+ unfold interp; simpl; fold (interp T) (interp U) (interp T') (interp U').
+ split.
+  destruct s2; simpl in H1.
+   destruct s1.
+    destruct s3; try discriminate.
+    destruct (eq_nat_dec (max n n0) n1); try discriminate.
+    subst n1.
+    apply typ_predicative_prod.
+     apply typ_type_cumul_le with n0; auto with *.
+     apply typ_type_cumul_le with n; auto with *.
+
+    destruct s3; try discriminate.
+    destruct (eq_nat_dec n n0); try discriminate.
+    subst n0.
+    apply typ_predicative_prod; trivial.
+    apply typ_type_cumul_le with 0; auto with *.
+    apply typ_prop_cumul; trivial.
+
+  destruct s3; try discriminate.
+  apply SN.typ_prod_prop; auto.
+  apply typ_sort_type_ok in H2; auto.
+
+  apply SN.eq_typ_prod; eauto.
+ (* Beta *)
+ destruct IHeq_typ1.
+ destruct IHeq_typ2.
+ destruct IHeq_typ3.
+ clear IHeq_typ4.
+ unfold interp; simpl; fold (interp T) (interp M) (interp U) (interp N).
+ split.
+  rewrite int_subst; fold (interp N); eauto.
+  fold (interp U).
+  apply SN.typ_beta_ok; auto.
+  apply typ_sort_type_ok in H6; auto.
+
+  rewrite int_subst; fold (interp N').
+  2:assert (h := Ty.typ_refl2 _ _ _ _ H); eauto.
+  apply SN.eq_typ_beta; eauto.
+ (* Red *)
+ destruct IHeq_typ1.
+ destruct IHeq_typ2.
+ split; trivial.
+ apply SN.typ_conv with (interp T); eauto.
+ (* Exp *)
+ destruct IHeq_typ1.
+ destruct IHeq_typ2.
+ split; trivial.
+ apply SN.typ_conv with (int_trm T'); eauto.
+ apply SN.sym; trivial.
+Qed.
+
+  Lemma interp_wf : forall e, Ty.wf e -> SN.wf (int_env e).
+induction e; simpl; intros.
+ apply SN.wf_nil.
+
+ inversion_clear H.
+ assert (wfe := Ty.typ_wf _ _ _ _ H0).
+ apply int_sound in H0.
+ destruct H0 as (H0,_).
+ apply SN.wf_cons_ok; auto.
+ apply typ_sort_type_ok in H0; auto.
+Qed.
+
+Lemma interp_sound : forall e M M' T,
+  Ty.eq_typ e M M' T ->
+  SN.wf (int_env e) /\ SN.typ (int_env e) (interp M) (interp T).
+intros.
+assert (wfe := Ty.typ_wf _ _ _ _ H).
+apply interp_wf in wfe.
+apply int_sound in H; destruct H; auto.
+Qed.
+
+(***********)
+(*
+----
+*)
+
+(** The main theorem: strong normalization of CC *)
+
+Lemma strong_normalization : forall e M M' T,
+  Ty.eq_typ e M M' T ->
+  Tm.sn M.
+Proof.
+intros.
+apply interp_sound in H.
+destruct H as (wfe,ty).
+apply SN.model_strong_normalization in ty; trivial.
+apply sn_sound; trivial.
+Qed.
+
+(* Print the assumptions made to derive strong normalization of ECC:
+   the axioms of ZF, and the existence of Grothendieck universes.
+   In fact we don't need full replacement, only the functional version,
+   so we have the SN theorem with only the axiom about Grothendieck universes.
+ *)
+Print Assumptions strong_normalization.
